verified array is sorted as well

resources/array_is_sorted/array_is_sorted_new.ml
@@ -1,0 +1,17 @@
+open Combinators
+
+let array_is_sorted (t: int array) =
+  let (len: int) = Array.length t in
+  if len = 0
+  then true
+  else
+    let (result: bool ref) = ref true in
+    let _ = while_downto (len - 1) 0 (fun (i: int) ->
+      let (elt: int) = t.(i) in
+      let (prev_elt: int) = t.(i - 1) in
+      if prev_elt > elt then
+        result := false;
+      !result
+    ) in
+    let (res: bool) = !result in
+    res
