resources/array_is_sorted/Verify_array_is_sorted_new.v
@@ -1,0 +1,70 @@
+Set Implicit Arguments.
+
+From CFML Require Import WPLib Stdlib.
+From TLC Require Import LibListZ.
+
+From Common Require Import Verify_combinators.
+From Common Require Import Tactics Solver Utils.
+
+From ProofsArrayIsSorted Require Import Array_is_sorted_new_ml.
+
+
+Lemma array_is_sorted_spec :
+  forall (a : array int) (l : list int),
+  SPEC (array_is_sorted a)
+  PRE (a ~> Array l)
+  POST (fun (b : bool) => \[b = is_sorted l] \* a ~> Array l).
+Proof using (All).
+  xcf.
+  xapp.
+  xif as cond.
+  - xvals*. { sis_list_solver. }
+  - xref result.
+    xletopaque tmp Htmp.
+    xapp (@while_downto_spec (length l - 1) 0 tmp
+            (fun (i: int) (b: bool) =>
+               \[ b = is_sorted (drop i l) ] \*
+                 result ~~> b \*
+                 a ~> Array l)
+         ). {
+      intros i Hi; apply Htmp; clear Htmp.
+      xpullpure Hexists.
+      xapp. { sis_handle_int_index_prove. }
+      xapp. { sis_handle_int_index_prove. }
+      xif;=> Hcond.
+      - xapp.
+        xapp.
+        xsimpl*. {
+          eapply (@not_is_sorted_gen _ 1);
+            rewrite ?length_drop_nonneg; rewrite ?read_drop;
+            try apply int_index_prove; try math.
+          math_rewrite (i - 1 + (1 - 1) = i - 1).
+          math_rewrite (i - 1 + 1 = i).
+          math.
+        }
+      - xval.
+        xapp.
+        xsimpl*. {
+          rewrite (@drop_cons_unfold _ Inhab_int); try math.
+          assert (l[i - 1] <= l[i]) by math.
+          apply is_sorted_gen;
+            math_rewrite (i - 1 + 1 = i);
+            auto;
+            try (rewrite <- Hexists; auto);
+            rewrite ?length_drop_nonneg; try math;
+            rewrite ?drop_drop, ?read_drop, Z.add_0_r;
+            auto; math.
+        }
+    } { math. } {  apply is_sorted_last_elt; auto; math. }
+    intros term i Hcond Heq.
+    xmatch.
+    xapp.
+    xvals*. {
+      symmetry in Heq; symmetry.
+      destruct term; simpl in Hcond; destruct Hcond as [Hlen Heq0].
+      - assert (Heq0last: i = 0) by (apply Z.eqb_eq; auto).
+        rewrite Heq0last in Heq; rewrite drop_zero in Heq; auto.
+      - rewrite <- (@list_eq_take_app_drop _ i l); try math.
+        rewrite is_sorted_app_r; auto.
+    }
+Qed.
